Add README file. Rework b2llvm_1.

FORMALISATION/b2llvm_1.thy
@@ -4,51 +4,31 @@ theory b2llvm_1
 imports Main
 begin
 
+section {* Syntax *}
+
+subsection {* Syntax for source B implementation *}
+
 text {* Definition of a type for B variables.*}
 
 type_synonym BVariable = string
 
 text {* Define the possible values taken by B variables. We make here the simplifying assumption 
-that such variables are integers. Needs to be extended to match the actual language. *}
+that such variables are integers. *}
 datatype BValue = BInt int
 
-text {* Definition of a (record) type for the state of the B component. The state is specified by
-a valuation of some variables, that we call the alphabet of the state. *}
-record BState =
-  alpha :: "BVariable set"         -- "alphabet for the state"
-  store :: "BVariable \<Rightarrow> BValue"   -- "valuation of the variables"
-
-text {* A type for B expressions. Needs to be extended to match the actual language. *}
+text {* A type for B expressions. *}
 datatype BExpr =
   Const BValue |
   BVar BVariable |
   Sum BExpr BExpr (infix "+\<^sub>B" 65)
-
-text {* The following definition gives an (operational) semantics of expressions. The evaluation of 
-an expression in a state yields a value. *}
-
-inductive BEvalExpr :: "BExpr \<times> BState \<Rightarrow>  BValue \<Rightarrow> bool" (infix "\<leadsto>\<^sub>B\<^sup>E" 55) where
-  "(Const v, _) \<leadsto>\<^sub>B\<^sup>E v" |
-  "(BVar v, \<sigma>) \<leadsto>\<^sub>B\<^sup>E store \<sigma> v" |
-  "\<lbrakk> (e1, \<sigma>) \<leadsto>\<^sub>B\<^sup>E BInt i1; (e2, \<sigma>) \<leadsto>\<^sub>B\<^sup>E BInt i2 \<rbrakk> \<Longrightarrow> (e1 +\<^sub>B e2, \<sigma>) \<leadsto>\<^sub>B\<^sup>E BInt (i1 + i2)"
 
 text {* A type for B instructions. Needs to be extended to match the actual language. *}
 datatype BInst =
   Asg BVariable BExpr (infix "\<leftarrow>" 60) |
   Blk "BInst list"
 
-text {* The "Concrete Semantics" textbook instead used predicates to specify big-step
-semantics. *}
-inductive
-  Bbig_step :: "BInst \<times> BState \<Rightarrow> BState \<Rightarrow> bool" (infix "\<leadsto>\<^sub>B" 55) and
-  Bbig_step_l :: "BInst list \<times> BState \<Rightarrow> BState \<Rightarrow> bool" (infix "\<leadsto>\<^sub>B\<^sup>*" 55)
-where
-  "\<lbrakk> (e, \<sigma>) \<leadsto>\<^sub>B\<^sup>E x \<rbrakk> \<Longrightarrow> (v \<leftarrow> e, \<sigma>) \<leadsto>\<^sub>B \<lparr> alpha = alpha \<sigma>, store = (store \<sigma>) (v := x) \<rparr>" |
-  "\<lbrakk> (il, \<sigma>) \<leadsto>\<^sub>B\<^sup>* \<sigma>' \<rbrakk> \<Longrightarrow> (Blk il, \<sigma>) \<leadsto>\<^sub>B \<sigma>'" |
-  
-  "( [], \<sigma>) \<leadsto>\<^sub>B\<^sup>* \<sigma>" |
-  "\<lbrakk> (i, \<sigma>) \<leadsto>\<^sub>B \<sigma>'; (il, \<sigma>') \<leadsto>\<^sub>B\<^sup>* \<sigma>'' \<rbrakk> \<Longrightarrow> (i # il, \<sigma>) \<leadsto>\<^sub>B\<^sup>* \<sigma>''"
-  
+subsection {* Syntax for target LLVM code *}
+
 text {* This completes the skeleton of a formal semantics of the B implementation language. 
 We next turn our attention to LLVM. First two types are introduced: they respectively 
 represent memory addresses and temporary variables.*}
@@ -56,13 +36,8 @@ represent memory addresses and temporary variables.*}
 type_synonym LAddr = nat
 type_synonym LTemp = nat
 
-text {* Again, we consider that values can only be integer values. Again this is a simplification
-so that we can initially focus on identifying an approach to model the translation from B to LLVM. *}
+text {* Again, we consider that values can only be integer values. *}
 datatype LValue = LInt int
-
-record LState =
-  mem :: "LAddr \<Rightarrow> LValue"    -- "models the global store"
-  local :: "LTemp \<Rightarrow> LValue"  -- "models the temporaries within LLVM functions"
 
 text {* Expressions in LLVM statements can only be constants or temporaries. They are
 formalized as follows: *}
@@ -70,32 +45,62 @@ datatype LExpr =
   Val LValue |                -- "literals"
   Var LTemp                   -- "temporaries"
 
-inductive LEvalExpr :: "LExpr \<times> LState \<Rightarrow> LValue \<Rightarrow> bool" (infix "\<leadsto>\<^sub>L\<^sup>E" 55) where
-  "(Val v, _) \<leadsto>\<^sub>L\<^sup>E v" |
-  "(Var v, \<sigma>) \<leadsto>\<^sub>L\<^sup>E (mem \<sigma>) v"
-  
-text {* Next, (a few) LLVM statements are formalized in the following type. Note that the typing 
-annotation found in the concrete syntax of LLVM is omitted (the formalization currently avoids 
-considering typing issues anyway). *}
-
 datatype LStm =
   Load LTemp LAddr |
   Store LExpr LAddr |
   Add LTemp LExpr LExpr
 
-text {* Follows the specification of the semantics for the selected LLVM statements. As with a
-B instruction, the semantics of a LLVM statement is a state transformer. *}
+text {* A LLVM program is a list of LLVM statements. *}
+type_synonym LProg = "LStm list"
 
-inductive
-  Lbig_step :: "LStm \<times> LState \<Rightarrow> LState \<Rightarrow> bool" (infix "\<leadsto>\<^sub>L" 55) and
-  Lbig_step_star :: "LStm list \<times> LState \<Rightarrow> LState \<Rightarrow> bool" (infix "\<leadsto>\<^sub>L\<^sup>*" 55)
+text {* I want to specify what is a well-formed LLVM program. Some properties that may be 
+expressed and proved are the following:
+\begin{itemize}
+\item the temporary names must form an increasing sequence of numbers, starting from 0;
+\item the program is well-typed;
+\item the program is in SSA form.
+\end{itemize}
+
+Proving each such property will require developing auxiliary definitions before addressing
+the corresponding proofs.
+*}
+
+(*
+type_synonym nat_list = "nat list"
+
+inductive is_nat_interval :: "nat \<Rightarrow> nat list \<Rightarrow> bool"
 where
-  "\<lbrakk> m = mem \<sigma> \<rbrakk> \<Longrightarrow> (Load t a, \<sigma>) \<leadsto>\<^sub>L \<lparr> mem = m, local = (local \<sigma>)(t := m a) \<rparr>" |
-  "\<lbrakk> (v, \<sigma>) \<leadsto>\<^sub>L\<^sup>E x \<rbrakk> \<Longrightarrow> (Store v a, \<sigma>) \<leadsto>\<^sub>L \<lparr> mem = (mem \<sigma>) (a := x), local = local \<sigma> \<rparr>" |
-  "\<lbrakk> (v1, \<sigma>) \<leadsto>\<^sub>L\<^sup>E (LInt i1); (v2, \<sigma>) \<leadsto>\<^sub>L\<^sup>E (LInt i2) \<rbrakk> \<Longrightarrow> 
-    (Add t v1 v2, \<sigma>) \<leadsto>\<^sub>L \<lparr> mem = (mem \<sigma>), local = (local \<sigma>)( t := LInt (i1 + i2) ) \<rparr>" |
-  "([], \<sigma>) \<leadsto>\<^sub>L\<^sup>* \<sigma>" |
-  "\<lbrakk> (s, \<sigma>) \<leadsto>\<^sub>L \<sigma>'; (sl, \<sigma>') \<leadsto>\<^sub>L\<^sup>* \<sigma>'' \<rbrakk> \<Longrightarrow> (s # sl, \<sigma>) \<leadsto>\<^sub>L\<^sup>* \<sigma>''"
+  "is_nat_interval n []" |
+  "\<lbrakk> is_nat_interval n (x # xl); x < n \<rbrakk> \<Longrightarrow> is_nat_interval n xl"
+
+fun upto :: "nat \<Rightarrow> nat list" where
+  "upto 0 = []" |
+  "upto (Suc n) = (upto n) @ [n]"
+
+lemma "is_nat_interval n (upto n)"
+sorry *)
+
+(*
+primrec LStm_temp :: "LStm \<Rightarrow> LTemp option" where
+  "LStm_temp (Load t a) = Some t" |
+  "LStm_temp (Store e a) = None" |
+  "LStm_temp (Add t e e') = Some t"
+
+primrec LProg_temp_first :: "LProg \<Rightarrow> LTemp option" where
+  "LProg_temp_first [] = None" |
+  "LProg_temp_first (i #il) = (if LStm_temp i = None then LProg_temp_first il else LStm_temp i)"
+
+primrec WF_LProg :: "LProg \<Rightarrow> bool" where
+  "WF_LProg [] = True" |
+  "WF_LProg (i # il) = ((WF_LProg il) \<and>
+                        (case (LStm_temp i, LProg_temp_first il) of
+                           (None, _) \<Rightarrow> True |
+                           (_, None) \<Rightarrow> True |
+                           (Some t1, Some t2) \<Rightarrow> t1 < t2))"
+                        
+*)
+
+subsection {* Generation of LLVM from B *}
 
 text {* The third part of the formalization deals with the generation of LLVM code from B
 expressions and instructions. All functions take as
@@ -118,30 +123,100 @@ definition WF_DataMap :: "DataMap \<Rightarrow> bool" where
 text {* The following function formalizes the encoding of B data into LLVM data. *}
 fun b2llvm_data :: "BValue \<Rightarrow> LValue" where
   "b2llvm_data (BInt i) = (LInt i)"
-  
-definition StateMap :: "BState \<Rightarrow> DataMap \<Rightarrow> LState \<Rightarrow> bool" where
-  "StateMap st\<^sub>B m st\<^sub>L \<equiv> \<forall> b v . b \<in> alpha st\<^sub>B \<longrightarrow> v = m b \<longrightarrow> b2llvm_data (store st\<^sub>B b) = mem st\<^sub>L v"
 
 text
 {*
 The first function formalizes the code generation for expressions:
  *}
-inductive 
-  b2llvm_expr :: "BExpr \<Rightarrow> DataMap \<Rightarrow> LTemp \<Rightarrow> (LStm list \<times> LExpr \<times> LTemp) \<Rightarrow> bool" (infix "\<Turnstile>\<^bsup>Expr\<^esup>" 50) 
+fun
+  b2llvm_expr :: "BExpr \<Rightarrow> DataMap \<Rightarrow> LTemp \<Rightarrow> (LStm list \<times> LExpr \<times> LTemp)" 
 where
-  "b2llvm_expr (Const (BInt i)) loc tmp ([], (Val (LInt i)), tmp)" |
-  "b2llvm_expr (BVar v) loc tmp ( [ Load tmp (loc v) ], Var tmp, tmp+1)" |
-  "\<lbrakk> b2llvm_expr e1 loc tmp (il1, v1, tmp1); 
-     b2llvm_expr e2 loc tmp1 (il2, v2, tmp2) \<rbrakk> \<Longrightarrow>
-      b2llvm_expr (e1 +\<^sub>B e2) loc tmp ( il1 @ il2 @ [ Add tmp2 v1 v2 ], Var tmp2, tmp2+1)"
+  "b2llvm_expr (Const (BInt i)) loc tmp = ([], (Val (LInt i)), tmp)" |
+  "b2llvm_expr (BVar v) loc tmp = ( [ Load tmp (loc v) ], Var tmp, tmp+1)" |
+  "b2llvm_expr (e1 +\<^sub>B e2) loc tmp =
+    (let (il1, v1, tmp1) = (b2llvm_expr e1 loc tmp) in
+       (let (il2, v2, tmp2) = (b2llvm_expr e2 loc tmp1) in
+         (il1 @ il2 @ [ Add tmp2 v1 v2 ], Var tmp2, tmp2+1)))"
 
-text
-{*
-  First, we want to express some properties about the translation of expressions.
-*}
-lemma b2llvm_exp_temporary_increase:
-  "b2llvm_expr e m tmp (sl, t, tmp') \<Longrightarrow> tmp \<le> tmp'"
-sorry
+text {* The following function formalizes the LLVM code generation from B instructions. *}
+
+inductive
+  b2llvm_stm :: "BInst \<times> DataMap \<times> LTemp \<Rightarrow> (LStm list \<times> LTemp) \<Rightarrow> bool" and
+  b2llvm_stm_list :: "BInst list \<times> DataMap \<times> LTemp \<Rightarrow> (LStm list \<times> LTemp) \<Rightarrow> bool"
+where
+  "\<lbrakk> b2llvm_expr e m tmp = (sl, e', t') \<rbrakk> \<Longrightarrow>
+  b2llvm_stm (v \<leftarrow> e, m, tmp) (sl @ [ Store e' (m v) ], t')" |
+  "\<lbrakk> b2llvm_stm_list (l, m, tmp) (sl, tmp') \<rbrakk> \<Longrightarrow>
+    b2llvm_stm (Blk l, m, tmp) (sl, tmp' )" |
+
+  "b2llvm_stm_list ([], m, tmp) ([], tmp)" |
+  "\<lbrakk> b2llvm_stm (i, m, tmp) (sl, tmp') ; 
+     b2llvm_stm_list(il, m, tmp') (sl', tmp'') \<rbrakk> \<Longrightarrow>
+   b2llvm_stm_list(i # il, m, tmp) (sl @ sl', tmp'')"
+
+section {* Semantics *}
+
+subsection {* Semantics for source B implementations *}
+
+text {* Definition of a (record) type for the state of the B component. The state is specified by
+a valuation of some variables, that we call the alphabet of the state. *}
+record BState =
+  alpha :: "BVariable set"         -- "alphabet for the state"
+  store :: "BVariable \<Rightarrow> BValue"   -- "valuation of the variables"
+
+text {* The following definition gives an (operational) semantics of expressions. The evaluation of 
+an expression in a state yields a value. *}
+
+fun BEvalExpr :: "BExpr \<times> BState \<Rightarrow>  BValue" where
+  "BEvalExpr (Const v, _) = v" |
+  "BEvalExpr (BVar v, \<sigma>) = store \<sigma> v" |
+  "BEvalExpr (e1 +\<^sub>B e2, \<sigma>) = (case (BEvalExpr (e1, \<sigma>), BEvalExpr(e2, \<sigma>)) of
+    (BInt i1, BInt i2) \<Rightarrow> BInt (i1 + i2))"
+
+text {* The "Concrete Semantics" textbook instead used predicates to specify big-step
+semantics. *}
+inductive
+  Bbig_step :: "BInst \<times> BState \<Rightarrow> BState \<Rightarrow> bool" (infix "\<leadsto>\<^sub>B" 55) and
+  Bbig_step_l :: "BInst list \<times> BState \<Rightarrow> BState \<Rightarrow> bool" (infix "\<leadsto>\<^sub>B\<^sup>*" 55)
+where
+  "(v \<leftarrow> e, \<sigma>) \<leadsto>\<^sub>B \<lparr> alpha = alpha \<sigma>, store = (store \<sigma>) (v := BEvalExpr(e, \<sigma>)) \<rparr>" |
+  "\<lbrakk> (il, \<sigma>) \<leadsto>\<^sub>B\<^sup>* \<sigma>' \<rbrakk> \<Longrightarrow> (Blk il, \<sigma>) \<leadsto>\<^sub>B \<sigma>'" |
+  
+  "( [], \<sigma>) \<leadsto>\<^sub>B\<^sup>* \<sigma>" |
+  "\<lbrakk> (i, \<sigma>) \<leadsto>\<^sub>B \<sigma>'; (il, \<sigma>') \<leadsto>\<^sub>B\<^sup>* \<sigma>'' \<rbrakk> \<Longrightarrow> (i # il, \<sigma>) \<leadsto>\<^sub>B\<^sup>* \<sigma>''"
+
+subsection {* Semantics for target LLVM code *}
+
+record LState =
+  mem :: "LAddr \<Rightarrow> LValue"    -- "models the global store"
+  local :: "LTemp \<Rightarrow> LValue"  -- "models the temporaries within LLVM functions"
+
+fun LEvalExpr :: "LExpr \<times> LState \<Rightarrow> LValue" where
+  "LEvalExpr (Val v, _) = v" |
+  "LEvalExpr (Var v, \<sigma>) = (mem \<sigma>) v"
+  
+text {* Next, (a few) LLVM statements are formalized in the following type. Note that the typing 
+annotation found in the concrete syntax of LLVM is omitted (the formalization currently avoids 
+considering typing issues anyway). *}
+
+text {* Follows the specification of the semantics for the selected LLVM statements. As with a
+B instruction, the semantics of a LLVM statement is a state transformer. *}
+
+inductive
+  Lbig_step :: "LStm \<times> LState \<Rightarrow> LState \<Rightarrow> bool" (infix "\<leadsto>\<^sub>L" 55) and
+  Lbig_step_star :: "LStm list \<times> LState \<Rightarrow> LState \<Rightarrow> bool" (infix "\<leadsto>\<^sub>L\<^sup>*" 55)
+where
+  "\<lbrakk> m = mem \<sigma> \<rbrakk> \<Longrightarrow> (Load t a, \<sigma>) \<leadsto>\<^sub>L \<lparr> mem = m, local = (local \<sigma>)(t := m a) \<rparr>" |
+  "(Store v a, \<sigma>) \<leadsto>\<^sub>L \<lparr> mem = (mem \<sigma>) (a := LEvalExpr(v, \<sigma>)), local = local \<sigma> \<rparr>" |
+  "\<lbrakk> LEvalExpr(v1, \<sigma>) = LInt i1; LEvalExpr (v2, \<sigma>) = LInt i2 \<rbrakk> \<Longrightarrow> 
+    (Add t v1 v2, \<sigma>) \<leadsto>\<^sub>L \<lparr> mem = (mem \<sigma>), local = (local \<sigma>)( t := LInt (i1 + i2) ) \<rparr>" |
+  "([], \<sigma>) \<leadsto>\<^sub>L\<^sup>* \<sigma>" |
+  "\<lbrakk> (s, \<sigma>) \<leadsto>\<^sub>L \<sigma>'; (sl, \<sigma>') \<leadsto>\<^sub>L\<^sup>* \<sigma>'' \<rbrakk> \<Longrightarrow> (s # sl, \<sigma>) \<leadsto>\<^sub>L\<^sup>* \<sigma>''"
+
+subsection {* Semantic aspects of code generation *}
+
+definition StateMap :: "BState \<Rightarrow> DataMap \<Rightarrow> LState \<Rightarrow> bool" where
+  "StateMap st\<^sub>B m st\<^sub>L \<equiv> \<forall> b v . b \<in> alpha st\<^sub>B \<longrightarrow> v = m b \<longrightarrow> b2llvm_data (store st\<^sub>B b) = mem st\<^sub>L v"
 
 text {*
   The following lemma states that executing the LLVM code corresponding to the evaluation of
@@ -159,7 +234,7 @@ text {*
 *}
 lemma b2llvm_expr_sound_mem: 
 assumes "StateMap \<sigma>\<^sub>B m \<sigma>\<^sub>L" and "WF_DataMap m" 
-and "(expB, m, tmp) \<Turnstile>\<^bsup>Expr\<^esup> (prog, expL, tmp')"
+and "b2llv_expr(expB, m, tmp) = (prog, expL, tmp')"
 and "(prog, \<sigma>\<^sub>L) \<leadsto>\<^sub>L\<^sup>* \<sigma>\<^sub>L'"
 shows
   "StateMap \<sigma>\<^sub>B m \<sigma>\<^sub>L'"
@@ -183,29 +258,13 @@ text {*
 *}
 lemma b2llvm_expr_sound_val: 
 assumes "StateMap \<sigma>\<^sub>B m \<sigma>\<^sub>L" and "WF_DataMap m" 
-and "(expB, m, tmp) \<Turnstile>\<^bsup>Expr\<^esup> (prog, expL, tmp')"
+and "b2llvm_expr expB m tmp = (prog, expL, tmp')"
 and "(prog, \<sigma>\<^sub>L) \<leadsto>\<^sub>L\<^sup>* \<sigma>\<^sub>L'"
-and "(expB, \<sigma>\<^sub>B) \<leadsto>\<^sub>B\<^sup>E valB"
-and "(expL, \<sigma>\<^sub>L') \<leadsto>\<^sub>L\<^sup>E valL"
+and "BEvalExpr (expB, \<sigma>\<^sub>B) =  valB"
+and "BEvalInst (expL, \<sigma>\<^sub>L') = valL"
 shows
   "b2llvm_data valB = valL"
 sorry
 
-text {* The following function formalizes the LLVM code generation from B instructions. *}
-
-inductive
-  b2llvm_stm :: "BInst \<times> DataMap \<times> LTemp \<Rightarrow> (LStm list \<times> LTemp) \<Rightarrow> bool" and
-  b2llvm_stm_list :: "BInst list \<times> DataMap \<times> LTemp \<Rightarrow> (LStm list \<times> LTemp) \<Rightarrow> bool"
-where
-  "\<lbrakk> (e, m, tmp) \<Turnstile>\<^bsup>Expr\<^esup> (sl, e', t') \<rbrakk> \<Longrightarrow>
-    b2llvm_stm (Asg v e, m, tmp) (sl @ [ Store e' (m v) ], t')" |
-  "\<lbrakk> b2llvm_stm_list (l, m, tmp) (sl, tmp') \<rbrakk> \<Longrightarrow>
-    b2llvm_stm (Blk l, m, tmp) (sl, tmp' )" |
-
-  "b2llvm_stm_list ([], m, tmp) ([], tmp)" |
-  "\<lbrakk> b2llvm_stm (i, m, tmp) (sl, tmp') ; 
-     b2llvm_stm_list(il, m, tmp') (sl', tmp'') \<rbrakk> \<Longrightarrow>
-   b2llvm_stm_list(i # il, m, tmp) (sl @ sl', tmp'')"
-   
 end
 
