FORMALISATION/README.md
@@ -1,0 +1,62 @@
+This directory contains the files related to a formal expression of the rules
+defining the code generation of LLVM code units from B implementations.
+
+This formalisation is incremental. Starting from a very small subset of the
+source B language, and gradually introducing more elements, we shall get as
+close as possible to the definition of the full system of rules. The different
+steps are the following:
+
+- Step 1:
+
+| Type system  | integers         |
+|--------------|------------------|
+| Expressions  | integer literals |
+|              | variables        |
+|              | sum              |
+|--------------|------------------|
+| Instructions | assignment       |
+|              | block            |
+|--------------|------------------|
+
+Specification of LLVM does not include typing annotations.
+
+- Step 2:
+
+| Type system  | integers           |
+|      	       | +Booleans	        |
+|--------------|--------------------|
+| Expressions  | integer literals   |
+|              | + Boolean literals |
+|              | variables          |
+|              | sum                |
+|--------------|--------------------|
+| Predicates   | + equalities       |
+|              | + conjunctions     |
+|              | + negations        |
+|--------------|--------------------|
+| Instructions | assignment         |
+|              | block              |
+|--------------|--------------------|
+
+Specification of LLVM does not include typing annotations.
+
+- Step 3:
+
+| Type system  | integers         |
+|      	       | Booleans	      |
+|--------------|------------------|
+| Expressions  | integer literals |
+|              | Boolean literals |
+|              | variables        |
+|              | sum              |
+|--------------|------------------|
+| Predicates   | equalities       |
+|              | conjunctions     |
+|              | negations        |
+|--------------|------------------|
+| Instructions | assignment       |
+|              | block            |
+|--------------|------------------|
+
++ Specification of LLVM does include typing annotations.
+
